NuBasicAbstractors.thy
@@ -88,6 +88,9 @@ lemma [simp]: " p \<nuLinkL> N <up-lift> f \<nuLinkR> x \<longleftrightarrow> (\
   unfolding UpLift_def Refining_ex by auto
 lemma [elim,\<nu>elim]: " x \<ratio> N <up-lift> f \<Longrightarrow> (\<And>y. f y = x \<Longrightarrow> y \<ratio> N \<Longrightarrow> C) \<Longrightarrow> C" unfolding Inhabited_def by auto
 
+lemma "\<^bold>c\<^bold>a\<^bold>s\<^bold>t x \<tycolon> N \<longmapsto> f x \<tycolon> N <up-lift> f" unfolding Cast_def by auto
+lemma "\<^bold>c\<^bold>a\<^bold>s\<^bold>t x \<tycolon> N \<longmapsto> f x \<tycolon> N <up-lift> f" unfolding Cast_def by auto
+
 lemma "\<nu>Equal (N <up-lift> f) can_eq eq \<longleftrightarrow> \<nu>Equal N (inv_imagep can_eq f) (inv_imagep eq f)"
   unfolding \<nu>Equal_def by (auto 0 6)
 
